x86/SymbtablegenSep.v
@@ -3123,19 +3123,19 @@ Proof.
 Qed.
 
 
-Lemma add_symb_to_list_id_eq: forall stbl id s,
-    In (id, s) (fold_left add_symb_to_list stbl []) ->
-    symbentry_id s = id.
-Proof.
-  induction stbl as [| e stbl].
-  - cbn. tauto.
-  - cbn. intros id s IN.
-    rewrite add_symb_to_list_inv in IN.
-    rewrite in_app in IN. destruct IN.
-    eauto.
-    unfold add_symb_to_list in H. 
-    inv H; try congruence. inv H0. 
-Qed.
+(* Lemma add_symb_to_list_id_eq: forall stbl id s, *)
+(*     In (id, s) (fold_left add_symb_to_list stbl []) -> *)
+(*     symbentry_id s = id. *)
+(* Proof. *)
+(*   induction stbl as [| e stbl]. *)
+(*   - cbn. tauto. *)
+(*   - cbn. intros id s IN. *)
+(*     rewrite add_symb_to_list_inv in IN. *)
+(*     rewrite in_app in IN. destruct IN. *)
+(*     eauto. *)
+(*     unfold add_symb_to_list in H.  *)
+(*     inv H; try congruence. inv H0.  *)
+(* Qed. *)
 
 
 Lemma link_symb_pres_id: forall s1 s2 s id,
@@ -3168,27 +3168,28 @@ Lemma link_symb_elements_entry_id_eq: forall stbl1 stbl2 id e,
                          (symbtable_to_tree stbl2))) ->
     symbentry_id e = id.
 Proof.
-  intros stbl1 stbl2 id e IN.
-  apply PTree.elements_complete in IN.
-  rewrite PTree.gcombine in IN; cbn; auto.
-  unfold link_symb_merge in IN.
-  destr_in IN. destr_in IN.
-  - apply PTree_Properties.in_of_list in Heqo.
-    apply PTree_Properties.in_of_list in Heqo0.
-    apply add_symb_to_list_id_eq in Heqo.
-    apply add_symb_to_list_id_eq in Heqo0.
-    erewrite (link_symb_pres_id s s0); eauto.
-    congruence.
-  - inv IN.
-    apply PTree_Properties.in_of_list in Heqo.
-    apply add_symb_to_list_id_eq in Heqo.
-    rewrite Heqo. 
-    auto.
-  - apply PTree_Properties.in_of_list in IN.
-    apply add_symb_to_list_id_eq in IN.
-    rewrite IN. 
-    auto.
-Qed.
+(*   intros stbl1 stbl2 id e IN. *)
+(*   apply PTree.elements_complete in IN. *)
+(*   rewrite PTree.gcombine in IN; cbn; auto. *)
+(*   unfold link_symb_merge in IN. *)
+(*   destr_in IN. destr_in IN. *)
+(*   - apply PTree_Properties.in_of_list in Heqo. *)
+(*     apply PTree_Properties.in_of_list in Heqo0. *)
+(*     apply add_symb_to_list_id_eq in Heqo. *)
+(*     apply add_symb_to_list_id_eq in Heqo0. *)
+(*     erewrite (link_symb_pres_id s s0); eauto. *)
+(*     congruence. *)
+(*   - inv IN. *)
+(*     apply PTree_Properties.in_of_list in Heqo. *)
+(*     apply add_symb_to_list_id_eq in Heqo. *)
+(*     rewrite Heqo.  *)
+(*     auto. *)
+(*   - apply PTree_Properties.in_of_list in IN. *)
+(*     apply add_symb_to_list_id_eq in IN. *)
+(*     rewrite IN.  *)
+(*     auto. *)
+(* Qed. *)
+Admitted.
 
 Lemma link_ordered_gen_symb_comm_syneq_size : forall p1 p2 stbl1 stbl2 dsz1 csz1 stbl2' dsz2 csz2 stbl3 dsz3 csz3 t' defs3,
     PTree_Properties.for_all (prog_option_defmap p1) (link_prog_check p1 p2) = true ->
@@ -3236,15 +3237,16 @@ Proof.
     destruct RELOC as (e' & stbl'' & RELOC & RS & EQ).
     subst.
     cbn.
-    rewrite acc_symb_ids_inv. rewrite rev_app_distr.
-    rewrite (acc_symb_ids_inv stbl''). rewrite rev_app_distr.
-    assert (acc_symb_ids [] e = acc_symb_ids [] e') as EQ.
-    { unfold acc_symb_ids.
-      erewrite reloc_symb_pres_id; eauto. 
-    }
-    rewrite EQ. f_equal.
-    eapply IHstbl; eauto.
-Qed.
+(*     rewrite acc_symb_ids_inv. rewrite rev_app_distr. *)
+(*     rewrite (acc_symb_ids_inv stbl''). rewrite rev_app_distr. *)
+(*     assert (acc_symb_ids [] e = acc_symb_ids [] e') as EQ. *)
+(*     { unfold acc_symb_ids. *)
+(*       erewrite reloc_symb_pres_id; eauto.  *)
+(*     } *)
+(*     rewrite EQ. f_equal. *)
+(*     eapply IHstbl; eauto. *)
+(* Qed. *)
+Admitted.
 
 
 Lemma link_ordered_gen_symb_comm : forall p1 p2 p stbl1 stbl2 dsz1 csz1 dsz2 csz2 f_ofs,
@@ -3664,12 +3666,13 @@ Lemma symbtable_to_tree_permutation_some: forall stbl stbl' id a,
 Proof.
   unfold symbtable_to_tree.
   intros stbl stbl' id a NORPT PERM ALL.
-  apply Permutation_pres_ptree_get_some with
-      (fold_left add_symb_to_list stbl []); eauto.
-  rewrite list_norepet_rev.
-  rewrite <- get_symbentry_ids_add_symb_eq. auto.
-  apply add_symb_to_list_permutation; auto.
-Qed.
+(*   apply Permutation_pres_ptree_get_some with *)
+(*       (fold_left add_symb_to_list stbl []); eauto. *)
+(*   rewrite list_norepet_rev. *)
+(*   rewrite <- get_symbentry_ids_add_symb_eq. auto. *)
+(*   apply add_symb_to_list_permutation; auto. *)
+(* Qed. *)
+Admitted.
 
 Lemma symbtable_to_tree_permutation_none: forall stbl stbl' id,
     Permutation stbl stbl' ->
@@ -3678,10 +3681,11 @@ Lemma symbtable_to_tree_permutation_none: forall stbl stbl' id,
 Proof.
   unfold symbtable_to_tree.
   intros stbl stbl' id PERM ALL.
-  apply Permutation_pres_ptree_get_none with
-      (fold_left add_symb_to_list stbl []); eauto.
-  apply add_symb_to_list_permutation; eauto.
-Qed.
+(*   apply Permutation_pres_ptree_get_none with *)
+(*       (fold_left add_symb_to_list stbl []); eauto. *)
+(*   apply add_symb_to_list_permutation; eauto. *)
+(* Qed. *)
+Admitted.
 
 Lemma link_symbtable_check_permutation: forall stbl stbl' id a,
     list_norepet (get_symbentry_ids stbl) ->
@@ -3764,21 +3768,23 @@ Proof.
   unfold symbtable_to_tree.
   apply Permutation_map.
   apply PTree_combine_permutation; auto.
-  - apply add_symb_to_list_permutation; auto.
-  - apply add_symb_to_list_permutation; auto.
+  - apply symbtable_to_idlist_permutation; auto.
+  - apply symbtable_to_idlist_permutation; auto.
   - rewrite get_symbentry_ids_add_symb_eq in l1.
     apply list_norepet_rev in l1.
     apply Permutation_pres_list_norepet with 
-        (map fst (fold_left add_symb_to_list stbl1' [])); auto.
+        (map fst (symbtable_to_idlist stbl1')); auto.
+    apply list_norepet_rev; eauto.
     apply Permutation_map. 
-    eapply add_symb_to_list_permutation; eauto.
+    eapply symbtable_to_idlist_permutation; eauto.
     apply Permutation_sym. auto.
   - rewrite get_symbentry_ids_add_symb_eq in l2.
     apply list_norepet_rev in l2.
     apply Permutation_pres_list_norepet with 
-        (map fst (fold_left add_symb_to_list stbl2' [])); auto.
-    apply Permutation_map. 
-    eapply add_symb_to_list_permutation; eauto.
+        (map fst (symbtable_to_idlist stbl2')); auto.
+    apply list_norepet_rev; eauto.
+    apply Permutation_map.     
+    eapply symbtable_to_idlist_permutation; eauto.
     apply Permutation_sym. auto.
 Qed.
   
